src/dafny/smart/intdiffalgo/incAlgoV5.dfy
@@ -14,6 +14,7 @@
  
 include "DiffTree.dfy"
 
+include "IncAlgoV1.dfy"
 include "IncAlgoV3.dfy"
 include "../trees/CompleteTrees.dfy"
 include "../synthattribute/ComputeRootPath.dfy"
@@ -24,6 +25,7 @@ include "../MerkleTrees.dfy"
 include "../paths/NextPathInCompleteTreesLemmas.dfy"
 include "../paths/PathInCompleteTrees.dfy"
 include "../seqofbits/SeqOfBits.dfy"
+include "../helpers/SeqHelpers.dfy"
 include "../trees/Trees.dfy"
 
 /**
@@ -32,6 +34,7 @@ include "../trees/Trees.dfy"
 module IncAlgoV5 {
  
     import opened DiffTree
+    import opened IncAlgoV1
     import opened IncAlgoV3
     import opened CompleteTrees
     import opened ComputeRootPath
@@ -41,71 +44,243 @@ module IncAlgoV5 {
     import opened NextPathInCompleteTreesLemmas
     import opened PathInCompleteTrees
     import opened SeqOfBits
+    import opened SeqHelpers
     import opened Trees
-
+    
     /**
-     *  @todo: division by power2 computation is assumed. Prove it.
      */
     method merkleV1(h : nat, k : nat, valOnLeftAt : seq<int>, seed: int) 
                                                         returns (r : int, next: seq<int>)
         requires 1 <= h == |valOnLeftAt|
-        requires k < power2(h)
+        //  make sure k % 2 == 0 at some point
+        requires k < power2(h) - 1
 
-        // ensures (r, next) == (computeRootPathDiffUp(natToBitList(k, h), valOnLeftAt, seed),
-        //     computeLeftSiblingOnNextPath(natToBitList(k, h), computeAllPathDiffUp(natToBitList(k, h), valOnLeftAt, seed), valOnLeftAt)
-        //     )
-
-        // ensures (r, next) == computeRootPathDiffAndLeftSiblingsUpv4(h, k, valOnLeftAt, seed)
-        // ensures r == computeRootPathDiffAndLeftSiblingsUpv4(h, k, valOnLeftAt, seed).0
+        ensures (r, next) == 
+            var p := natToBitList(k, h);
+            (
+                computeRootPathDiffUp(p, valOnLeftAt, seed),
+                computeLeftSiblingOnNextPath(p, 
+                    computeAllPathDiffUp(p, valOnLeftAt, seed), 
+                    valOnLeftAt
+                )
+        )
     {
         var i := 0;
-        var k' := k;
+        var k' : nat := k;
 
         r := seed ;
         next := [] ; 
 
-        ghost var h1 := h;
-        ghost var (r', next') := computeRootPathDiffAndLeftSiblingsUpv4c(h, k, valOnLeftAt, seed, []);
+        ghost var h1 : nat := h;
+        ghost var (r', next') := computeRootPathDiffAndLeftSiblingsUpv4d(h, k, valOnLeftAt, seed, []);
 
-        //  need this fact to prove next assert
-        assert(valOnLeftAt == valOnLeftAt[..h - i]);
+        //  compute natToBitList(k, h)
+        ghost var p : seq<bit> := [];
 
-        while (i < h)
+        //  need this fact to prove main loop invariant holds on entry
+        assert(valOnLeftAt == take(valOnLeftAt, h - i));
+
+        while (i < h && k' % 2 == 1)
 
             invariant 0 <= i <= h
-            invariant i == |valOnLeftAt[.. i]|
+            invariant i == |take(valOnLeftAt, i)|
             invariant 0 <= k' < power2(h1)
             invariant h1 == h - i
-            invariant (r', next') == computeRootPathDiffAndLeftSiblingsUpv4c(h1, k', valOnLeftAt[..h1], r, next);
+            //  Main invariant
+            invariant (r', next') == 
+                computeRootPathDiffAndLeftSiblingsUpv4d(h1, k', take(valOnLeftAt, h1), r, next);
 
+            //  p invariant
+            invariant |p| == i
+            invariant forall k :: 0 <= k < |p| ==> p[k] == 1
+
+            //  Value of natToBitList2(k, h)
+            invariant natToBitList2(k, h) == natToBitList2(k', h1) + p
 
             decreases h - i 
-        {
-            if k' % 2 == 0 {
-                next := [r] + next ;
-                r := diff(r, 0);
-            } else {
-                next := [valOnLeftAt[h - i - 1]] + next ;
-                r := diff(valOnLeftAt[h - i - 1], r);
+        { 
+            p := [1] + p;
+            next := [valOnLeftAt[h - i - 1]] + next ;
+            r := diff(valOnLeftAt[h - i - 1], r);
+            //  the following is used to prove the main invariant
+            // assert(valOnLeftAt[..h1 - 1] == valOnLeftAt[..h1][..h1 - 1]);
+            calc == {
+                take(valOnLeftAt, h1 - 1);
+                take(take(valOnLeftAt, h1), h1 - 1);
             }
-            //  the following is used to prove Inv4
-            assert(valOnLeftAt[..h1 - 1] == valOnLeftAt[..h1][..h1 - 1]);
+
             i := i + 1;
             k' := k' / 2;
             h1 := h1 - 1;
         }
-        //  after the loop we get the result
+
         assert(
-            (r, next) // == (r', next')
-            ==
-            computeRootPathDiffAndLeftSiblingsUpv4c(h, k, valOnLeftAt, seed, [])
+            (r', next') == 
+                computeRootPathDiffAndLeftSiblingsUpv4d(h1, k', take(valOnLeftAt, h1), r, next)
         );
+        
+        //  Use lemma to prove that h1 >= 1
+        calc ==> {
+            true;
+            { foo222(h, h1, k, k', p); }
+            h1 >= 1;
+        }       
+        assert(h1 >= 1);
+
+        assert(k' % 2 == 0);
+
+        //  use path as an interndediate to prove that 
+        // r ' ==  computeRootPathDiffUpv3(1, k', take(valOnLeftAt, h1), r) 
+        assert( k' < power2(h1));
+        ghost var pa : seq<bit> := natToBitList(k', h1);
+        calc == {
+            r';
+            computeRootPathDiffAndLeftSiblingsUpv4d(h1, k', take(valOnLeftAt, h1), r, next).0;
+            { computeRootAndSiblingsV4dIsCorrect(h1, k', take(valOnLeftAt, h1), r, next) ; }
+            computeRootPathDiffAndLeftSiblingsUpv4b(h1, k', take(valOnLeftAt, h1), r).0 ;
+            { computeRootAndSiblingsV4bIsCorrect(h1, k',  take(valOnLeftAt, h1), r) ; }
+            computeRootPathDiffAndLeftSiblingsUpv4(h1, k',  take(valOnLeftAt, h1), r).0;
+            { computeRootAndSiblingsV4IsCorrect(h1, k', take(valOnLeftAt, h1), r ) ; }
+            computeRootPathDiffUp(pa, take(valOnLeftAt, h1), r );
+            { v3computesRootPath(h1, k', take(valOnLeftAt, h1), r); }
+            computeRootPathDiffUpv3(h1, k', take(valOnLeftAt, h1), r);
+        }
+       
+        //  new invariant should be
+        assert( r' ==
+            computeRootPathDiffUpv3(h1, k', take(valOnLeftAt, h1), r)
+        );
+        calc == {
+            computeRootPathDiffUpv3(h1, k', take(valOnLeftAt, h1), r);
+            calc == {
+                init(take(valOnLeftAt, h1));
+                take(valOnLeftAt, h1 - 1);
+            }
+            computeRootPathDiffUpv3(h1 - 1, k' / 2, take(valOnLeftAt, h1 - 1), diff(r, 0));
+        }
+        //  k' % 2 == 1
+        next := take(valOnLeftAt, h - i - 1) + [r] + next ;
+        // next := [r] + next ;
+        r := diff(r, 0);
+        i := i + 1;
+        k' := k' / 2;
+        h1 := h1 - 1;
+
+        //  next computation is complete
+        assert(
+            next == next'
+        );
+       
+
+       assert( r' ==
+            computeRootPathDiffUpv3(h1, k', take(valOnLeftAt, h1), r)
+        );
+        //  Show that computation of root path is OK
+        assert(i >= 0);
+        //  Now compute root path only
+        while ( i < h ) 
+            invariant i >= 0;
+            invariant 0 <= i <= h
+            invariant h1 == h - i
+            invariant h1 == |take(valOnLeftAt, h1)|
+            invariant k' < power2(h1)
+            invariant r' ==  computeRootPathDiffUpv3(h1, k', take(valOnLeftAt, h1), r)
+
+        {
+            if k' % 2 == 0 {
+                r := diff(r, 0);
+            } else {
+                r := diff(valOnLeftAt[h - i - 1], r);
+            }
+            calc == {
+                take(valOnLeftAt, h1 - 1);
+                take(take(valOnLeftAt, h1), h1 - 1);
+            }
+            i := i + 1;
+            k' := k' / 2;
+            h1 := h1 - 1;
+            
+        }
+        assert(r' == r);
+        assert(next == next');
+        calc == {
+            (r, next);
+            computeRootPathDiffAndLeftSiblingsUpv4d(h, k, valOnLeftAt, seed, []);
+            { computeRootAndSiblingsV4dIsCorrect(h, k, valOnLeftAt, seed, []) ; }
+            computeRootPathDiffAndLeftSiblingsUpv4b(h, k, valOnLeftAt, seed);
+            { computeRootAndSiblingsV4bIsCorrect(h, k, valOnLeftAt, seed) ; }
+            computeRootPathDiffAndLeftSiblingsUpv4(h, k, valOnLeftAt, seed);
+            { computeRootAndSiblingsV4IsCorrect(h, k, valOnLeftAt, seed) ; }
+            (computeRootPathDiffUp(natToBitList(k, h), valOnLeftAt, seed),
+            computeLeftSiblingOnNextPath(natToBitList(k, h), computeAllPathDiffUp(natToBitList(k, h), valOnLeftAt, seed), valOnLeftAt)
+            );
+        }
+
     }
 
-    lemma divIsZero(n : nat, m : nat) 
-        requires n < m
-        ensures n / m == 0 
+    method test1(k : nat, h : nat)
+         requires k < power2(h) - 1
     {
+        var i := 0;
+        var k' : nat := k;
+        ghost var p : seq<bit> := [];
+        ghost var h1 : nat := h;
+        
+        while ( i < h && k' % 2 == 1)
+            invariant 0 <= i <= h
+            invariant 0 <= k' < power2(h1)
+            invariant h1 == h - i
+            invariant natToBitList2(k, h) == natToBitList2(k', h1) + p
+            invariant forall k :: 0 <= k < |p| ==> p[k] == 1
+        {
+            p := [1] + p;
+            i := i + 1;
+            k' := k' / 2;
+            h1 := h1 - 1;
+        }
 
+        //  Loop invariant
+        // assert(natToBitList2(k, h) == natToBitList2(k', h1) + p);
+        //  now show that h1 >=1 necesserily
+        calc ==> {
+            // k < power2(h) - 1 && k < power2(h1);
+            true;
+            { foo222(h, h1, k, k', p); }
+            h1 >= 1;
+        }
+        assert(h1 >= 1);
+    }   
+
+
+    /**
+     *  If R2 and R3 hold, then necesseraly h1 >= 1.   
+     */
+    lemma {:induction h, h1, k} foo222(h: nat, h1: nat, k: nat, k' : nat, p : seq<bit>) 
+        requires k < power2(h) - 1
+        requires k' < power2(h1)
+        requires natToBitList2(k, h) == natToBitList2(k', h1) + p    //  R2
+        requires forall k :: 0 <= k < |p| ==> p[k] == 1             //  R3
+        ensures  h1 >= 1
+    {
+        if (h1 == 0) {
+            calc == {
+                k;
+                { bitToNatToBitsIsIdentity(k, h) ;}
+                bitListToNat(natToBitList2(k, h));
+                bitListToNat(natToBitList2(k', h1) + p);
+                bitListToNat(natToBitList2(k', 0) + p);
+                bitListToNat([] + p);
+                calc == {
+                    [] + p;
+                    p;
+                }
+                bitListToNat(p);
+                { valueOfSeqOfOnes(p); }
+                power2(|p|) - 1;
+                power2(h) - 1;
+            }
+        }
+        assert(h1 >= 1);
     }
+
  }
